Make label functions opaque to SMT

src/DY.Core.Label.fst
@@ -42,41 +42,90 @@ val is_corrupt_order:
   [SMTPat (is_corrupt tr who1); SMTPat (who1 `pre_pre_label_order.rel` who2)]
 let is_corrupt_order tr who1 who2 = ()
 
+[@@"opaque_to_smt"]
 val can_flow: trace -> label -> label -> prop
 let can_flow tr l1 l2 =
   l2 `(label_order (is_corrupt tr)).rel` l1
 
+[@@"opaque_to_smt"]
 val secret: label
 let secret =
   DY.Core.Label.Lattice.Leaf Secret
 
+[@@"opaque_to_smt"]
 val public: label
 let public =
   DY.Core.Label.Lattice.Leaf Public
 
+[@@"opaque_to_smt"]
 val meet: label -> label -> label
 let meet l1 l2 =
   DY.Core.Label.Lattice.Meet l1 l2
 
+[@@"opaque_to_smt"]
 val join: label -> label -> label
 let join l1 l2 =
   DY.Core.Label.Lattice.Join l1 l2
 
+[@@"opaque_to_smt"]
 val principal_label: principal -> label
 let principal_label prin =
   DY.Core.Label.Lattice.Leaf (State (P prin))
 
+[@@"opaque_to_smt"]
 val principal_state_label: principal -> nat -> label
 let principal_state_label prin sess_id =
   DY.Core.Label.Lattice.Leaf (State (S prin sess_id))
 
+[@@"opaque_to_smt"]
 val principal_corrupt: trace -> principal -> prop
 let principal_corrupt tr prin =
   is_corrupt tr (P prin)
 
+[@@"opaque_to_smt"]
 val principal_state_corrupt: trace -> principal -> nat -> prop
 let principal_state_corrupt tr prin sess_id =
   is_corrupt tr (S prin sess_id)
+
+val principal_label_injective:
+  p1:principal -> p2:principal ->
+  Lemma
+  (requires principal_label p1 == principal_label p2)
+  (ensures p1 == p2)
+  [SMTPat (principal_label p1); SMTPat (principal_label p2)]
+let principal_label_injective p1 p2 =
+  normalize_term_spec principal_label
+
+val principal_state_label_injective:
+  p1:principal -> s1:nat -> p2:principal -> s2:nat ->
+  Lemma
+  (requires principal_state_label p1 s1 == principal_state_label p2 s2)
+  (ensures p1 == p2 /\ s1 == s2)
+  [SMTPat (principal_state_label p1 s1); SMTPat (principal_state_label p2 s2)]
+let principal_state_label_injective p1 s1 p2 s2 =
+  normalize_term_spec principal_state_label
+
+val principal_corrupt_later:
+  tr1:trace -> tr2:trace ->
+  prin:principal ->
+  Lemma
+  (requires principal_corrupt tr1 prin /\ tr1 <$ tr2)
+  (ensures principal_corrupt tr2 prin)
+  [SMTPat (principal_corrupt tr1 prin); SMTPat (tr1 <$ tr2)]
+let principal_corrupt_later tr1 tr2 prin =
+  assert_norm(principal_corrupt tr1 prin == is_corrupt tr1 (P prin));
+  assert_norm(principal_corrupt tr2 prin == is_corrupt tr2 (P prin))
+
+val principal_state_corrupt_later:
+  tr1:trace -> tr2:trace ->
+  prin:principal -> sess_id:nat ->
+  Lemma
+  (requires principal_state_corrupt tr1 prin sess_id /\ tr1 <$ tr2)
+  (ensures principal_state_corrupt tr2 prin sess_id)
+  [SMTPat (principal_state_corrupt tr1 prin sess_id); SMTPat (tr1 <$ tr2)]
+let principal_state_corrupt_later tr1 tr2 prin sess_id =
+  assert_norm(principal_state_corrupt tr1 prin sess_id == is_corrupt tr1 (S prin sess_id));
+  assert_norm(principal_state_corrupt tr2 prin sess_id == is_corrupt tr2 (S prin sess_id))
 
 val can_flow_reflexive:
   tr:trace -> l:label ->
@@ -84,6 +133,7 @@ val can_flow_reflexive:
   (ensures l `can_flow tr` l)
   [SMTPat (l `can_flow tr` l)]
 let can_flow_reflexive tr l =
+  normalize_term_spec can_flow;
   (label_order (is_corrupt tr)).refl l
 
 val can_flow_transitive:
@@ -93,6 +143,7 @@ val can_flow_transitive:
   (ensures l1 `can_flow tr` l3)
   [SMTPat (l1 `can_flow tr` l3); SMTPat (l1 `can_flow tr` l2)]
 let can_flow_transitive tr l1 l2 l3 =
+  normalize_term_spec can_flow;
   (label_order (is_corrupt tr)).trans l3 l2 l1
 
 val can_flow_later:
@@ -103,6 +154,7 @@ val can_flow_later:
   (ensures l1 `can_flow tr2` l2)
   [SMTPat (l1 `can_flow tr1` l2); SMTPat (tr1 <$ tr2)]
 let can_flow_later tr1 tr2 l1 l2 =
+  normalize_term_spec can_flow;
   DY.Core.Label.Lattice.lattice_order_monotone (pre_label_order pre_pre_label_order (is_corrupt tr1)) (pre_label_order pre_pre_label_order (is_corrupt tr2)) l2 l1
 
 val secret_is_bottom:
@@ -111,6 +163,8 @@ val secret_is_bottom:
   (ensures l `can_flow tr` secret)
   [SMTPat (l `can_flow tr` secret)]
 let secret_is_bottom tr l =
+  normalize_term_spec can_flow;
+  normalize_term_spec secret;
   DY.Core.Label.Lattice.bottom_to_bottom (pre_label_order pre_pre_label_order (is_corrupt tr)) Secret l
 
 val public_is_top:
@@ -119,6 +173,8 @@ val public_is_top:
   (ensures public `can_flow tr` l)
   [SMTPat (public `can_flow tr` l)]
 let public_is_top tr l =
+  normalize_term_spec can_flow;
+  normalize_term_spec public;
   DY.Core.Label.Lattice.top_to_top (pre_label_order pre_pre_label_order (is_corrupt tr)) Public l
 
 val meet_eq:
@@ -127,6 +183,8 @@ val meet_eq:
   (ensures meet y1 y2 `can_flow tr` x <==> (y1 `can_flow tr` x /\ y2 `can_flow tr` x))
   [SMTPat (meet y1 y2 `can_flow tr` x)] //Not sure about this
 let meet_eq tr x y1 y2 =
+  normalize_term_spec can_flow;
+  normalize_term_spec meet;
   DY.Core.Label.Lattice.meet_eq (pre_label_order pre_pre_label_order (is_corrupt tr)) x y1 y2
 
 val join_eq:
@@ -135,6 +193,8 @@ val join_eq:
   (ensures y `can_flow tr` join x1 x2 <==> (y `can_flow tr` x1 /\ y `can_flow tr` x2))
   [SMTPat (y `can_flow tr` join x1 x2)] //Not sure about this
 let join_eq tr x1 x2 y =
+  normalize_term_spec can_flow;
+  normalize_term_spec join;
   DY.Core.Label.Lattice.join_eq (pre_label_order pre_pre_label_order (is_corrupt tr)) x1 x2 y
 
 val principal_flow_to_public_eq:
@@ -143,6 +203,10 @@ val principal_flow_to_public_eq:
   (ensures (principal_label prin) `can_flow tr` public <==> principal_corrupt tr prin)
   [SMTPat ((principal_label prin) `can_flow tr` public)] //Not sure about this
 let principal_flow_to_public_eq tr prin =
+  normalize_term_spec can_flow;
+  normalize_term_spec principal_label;
+  normalize_term_spec public;
+  assert_norm(principal_corrupt tr prin == is_corrupt tr (P prin));
   DY.Core.Label.Lattice.leaf_eq (pre_label_order pre_pre_label_order (is_corrupt tr)) Public (State (P prin))
 
 val principal_state_flow_to_public_eq:
@@ -151,6 +215,10 @@ val principal_state_flow_to_public_eq:
   (ensures (principal_state_label prin sess_id) `can_flow tr` public <==> principal_state_corrupt tr prin sess_id)
   [SMTPat ((principal_state_label prin sess_id) `can_flow tr` public)] //Not sure about this
 let principal_state_flow_to_public_eq tr prin sess_id =
+  normalize_term_spec can_flow;
+  normalize_term_spec principal_state_label;
+  normalize_term_spec public;
+  assert_norm(principal_state_corrupt tr prin sess_id == is_corrupt tr (S prin sess_id));
   DY.Core.Label.Lattice.leaf_eq (pre_label_order pre_pre_label_order (is_corrupt tr)) Public (State (S prin sess_id))
 
 val principal_flow_to_principal_state:
@@ -158,7 +226,10 @@ val principal_flow_to_principal_state:
   Lemma
   (ensures (principal_label prin) `can_flow tr` (principal_state_label prin sess_id))
   [SMTPat ((principal_label prin) `can_flow tr` (principal_state_label prin sess_id))]
-let principal_flow_to_principal_state tr prin sess_id = ()
+let principal_flow_to_principal_state tr prin sess_id =
+  normalize_term_spec can_flow;
+  normalize_term_spec principal_label;
+  normalize_term_spec principal_state_label
 
 val join_flow_to_public_eq:
   tr:trace -> x1:label -> x2:label ->
@@ -166,4 +237,7 @@ val join_flow_to_public_eq:
   (ensures (join x1 x2) `can_flow tr` public <==> x1 `can_flow tr` public \/ x2 `can_flow tr` public)
   [SMTPat ((join x1 x2) `can_flow tr` public)] //Not sure about this
 let join_flow_to_public_eq tr x1 x2 =
+  normalize_term_spec can_flow;
+  normalize_term_spec join;
+  normalize_term_spec public;
   DY.Core.Label.Lattice.leaf_less_join (pre_label_order pre_pre_label_order (is_corrupt tr)) Public x1 x2
